src/cbor/pulse/CBOR.Pulse.API.Base.fst
@@ -477,12 +477,12 @@ let map_iterator_next_t
   (#z: Ghost.erased (list (cbor & cbor))) ->
   stt t
     (R.pts_to x y ** iter py y z ** pure (Cons? z))
-    (fun res -> exists* p' v' y' z' .
+    (fun res -> exists* py' p' v' y' z' .
       vmatch2 p' res v' **
       R.pts_to x y' **
-      iter py y' z' **
+      iter py' y' z' **
       Trade.trade
-        (vmatch2 p' res v' ** iter py y' z')
+        (vmatch2 p' res v' ** iter py' y' z')
         (iter py y z) **
       pure (Ghost.reveal z == v' :: z')
     )
